FormalUrchin/test_compile.lean
@@ -1,0 +1,19 @@
+import FormalUrchin.compile
+
+def testProgram : mir.Prog :=
+  Lean.AssocList.empty.insert 0 [mir.Stmt.Assgn [2] (mir.RExpr.CopyOp [1]), mir.Stmt.Halt]
+
+
+  def test_placemap := Lean.AssocList.empty.insert 1 (TyVal.NatTy, oseair.Register.P 0)
+
+  def test_CompileBB : IO Unit :=
+    let ctx : compiler.CompileCtx := { placemap := test_placemap, prog := Lean.AssocList.empty.insert 0 [], regSuffix := 1, currBB := 0 }
+    let result := compiler.CompileBB testProgram 0 ctx
+    match result with
+    | compiler.CompileResult.Ok cctx => IO.println cctx.prog
+    | compiler.CompileResult.Err msg => IO.println msg
+
+    def main : IO Unit :=
+      test_CompileBB
+
+    #eval main
